now define leaf as node with two empty children

projet.v
@@ -5,34 +5,26 @@ Open Scope Z_scope.
 
 Inductive AB : Set :=
   | Node : Z -> AB -> AB -> AB
-  | Leaf : Z -> AB
   | Empty : AB.
-
-Definition node_value (a : AB) : option Z :=
-  match a with
-  | (Node v _ _) => Some v
-  | (Leaf v) => Some v
-  | Empty => None 
-end.
 
 Inductive is_ABR : AB -> Prop :=
   | Is_Empty : is_ABR Empty
-  | Is_Leaf : forall v : Z, is_ABR (Leaf v)
-  | Node_Both : forall (v vl vr : Z) (al ar : AB), is_ABR al -> is_ABR ar ->
-    Some vl = (node_value al) -> Some vr = (node_value ar) -> vl <= v -> v <= vr ->
+  | Is_Leaf : forall v : Z, is_ABR (Node v Empty Empty)
+  | Node_Both : forall (v vl vr : Z) (al ar sall salr sarl sarr : AB), is_ABR al -> is_ABR ar ->
+    al = (Node vl sall salr) -> ar = (Node vr sarl sarr) -> vl <= v -> v <= vr ->
     is_ABR (Node v al ar)
-  | Node_Left : forall (v vl : Z) (al : AB), is_ABR al -> Some vl = (node_value al) ->
+  | Node_Left : forall (v vl : Z) (al sal sar : AB), is_ABR al -> al = (Node vl sal sar) ->
     vl <= v -> is_ABR (Node v al Empty)
-  | Node_Right : forall (v vr : Z) (ar : AB), is_ABR ar -> Some vr = (node_value ar) ->
+  | Node_Right : forall (v vr : Z) (ar sal sar : AB), is_ABR ar -> ar = (Node vr sal sar) ->
     v <= vr -> is_ABR (Node v Empty ar).
 
-Definition benchmark_01 := (Node 3 (Node 1 (Leaf 0) (Leaf 3)) (Leaf 5)).
-Definition benchmark_02 := (Node 5 (Node 3 (Leaf 2) (Leaf 3)) (Node 7 (Leaf 7) (Leaf 8))).
-Definition benchmark_03 := (Node 15 (Node 12 (Node 11 (Leaf 5) Empty) (Node 14 (Node 12 Empty (Leaf 13)) (Leaf 15))) (Node 18 (Leaf 17) (Node 19 Empty (Leaf 20)))).
+Definition benchmark_01 := (Node 3 (Node 1 (Node 0 Empty Empty) (Node 3 Empty Empty)) (Node 5 Empty Empty)).
+Definition benchmark_02 := (Node 5 (Node 3 (Node 2 Empty Empty) (Node 3 Empty Empty)) (Node 7 (Node 7 Empty Empty) (Node 8 Empty Empty))).
+Definition benchmark_03 := (Node 15 (Node 12 (Node 11 (Node 5 Empty Empty) Empty) (Node 14 (Node 12 Empty (Node 13 Empty Empty)) (Node 15 Empty Empty))) (Node 18 (Node 17 Empty Empty) (Node 19 Empty (Node 20 Empty Empty)))).
 
 Lemma p1 : is_ABR benchmark_01.
-apply (Node_Both _ 1 5).
-apply (Node_Both _ 0 3).
+eapply Node_Both.
+eapply Node_Both.
 apply Is_Leaf.
 apply Is_Leaf.
 auto.
@@ -45,19 +37,44 @@ auto.
 omega.
 omega.
 Qed.
+
+Ltac apply_is_ABR :=
+  repeat
+  apply Is_Empty || apply Is_Leaf || eapply Node_Right ||
+  eapply Node_Left || eapply Node_Both || auto || omega.
 
 Lemma p2 : is_ABR benchmark_02.
-apply (Node_Both _ 3 7).
-apply (Node_Both _ 2 3).
+apply_is_ABR.
+Qed.
+
+
+Lemma p3 : is_ABR benchmark_03.
+eapply Node_Both.
+eapply Node_Both.
+eapply Node_Left.
+eapply Is_Leaf.
+auto.
+omega.
+eapply Node_Both.
+eapply Node_Right.
 apply Is_Leaf.
+auto.
+omega.
 apply Is_Leaf.
 auto.
 auto.
 omega.
 omega.
-apply (Node_Both _ 7 8).
+auto.
+auto.
+omega.
+omega.
+eapply Node_Both.
 apply Is_Leaf.
+eapply Node_Right.
 apply Is_Leaf.
+auto.
+omega.
 auto.
 auto.
 omega.
@@ -68,4 +85,8 @@ omega.
 omega.
 Qed.
 
-Lemma
+Lemma p4 : is_ABR benchmark_03.
+apply_is_ABR.
+Qed.
+
+Fixpoint insert
